made L4 to L4a faster : 40s to 0.002s (Eval compute)
Eval vm_compute was fast even before the change (0.003s), and is still so.
Used another implementation debruijn to named conversion which has N log N complexity (linear if +,- on numbers is constant time).
However, the main bottleneck was somewhere else -- in SquiggleEq term representation!

It was using a "bundled"[1, Sec. 3] approach where each (sub)term has the whole description of the language (including recursive functions denoting the signature of operators, decidable equality of operators) as an implicit argument.
Now, it is almost totally unbundled. The type of operators is the only implicit argument in (sub)terms.

The SquiggleEq LIBRARY NEEDS TO BE REBUILT. Execute make -j 4 at the root of the repository (parent of theories/).

[1]: Spitters, Bas, and Eelis Van Der Weegen. “Type Classes for Mathematics in Type Theory.” MSCS 21, no. Special Issue 04 (2011): 795–825. doi:10.1017/S0960129511000119.
http://arxiv.org/pdf/1102.1323v1.pdf

certicoq/libraries/SquiggleEq/terms.v
@@ -18,10 +18,9 @@ Require Import Recdef.
 Require Import Eqdep_dec.
 Require Import varInterface.
 
-Class GenericTermSig : Type :=
+Class GenericTermSig (Opid : Type) : Type :=
 {
 (** the collection of operators in the language. For example, in lambda calculus, App and Lam are operators *)
-  Opid : Set;
 (** Arities for each operator. An [Opid] [o] takes 
   [length (OpBindings o)] arguments. The number of bound variables in the ith argument is 
   specified by the ith member of [(OpBindings o)].
@@ -29,12 +28,13 @@ Class GenericTermSig : Type :=
   A lambda takes one argument and that argument binds 1 variable. An application takes 2 arguments,
   each of which bind 0 variables.*)
   OpBindings : Opid -> list nat;
-  opid_dec : forall x y : Opid, {x = y} + {x <> y};
 }.
 
+Generalizable Variable Opid.
 
 Section terms.
-Context {NVar VarClass} `{VarType NVar VarClass} {gts : GenericTermSig}.
+
+Context {NVar VarClass} `{VarType NVar VarClass} `{Deq Opid} {gts : GenericTermSig Opid}.
 
 Inductive NTerm : Type :=
 | vterm: NVar -> NTerm
@@ -216,36 +216,37 @@ https://coq.inria.fr/bugs/show_bug.cgi?id=3343
 
 (** Just decidability of equality on variables suffices for these definitions.
   The full [VarType] may not be needed until [ssubst]*)
-Fixpoint free_vars {NVar} `{Deq NVar} {gts : GenericTermSig}  
+Fixpoint free_vars {NVar} `{Deq NVar} {Opid:Type}
   (t:NTerm) {struct t}: list NVar :=
   match t with
   | vterm v => [v]
-  | oterm op bts => flat_map (@free_vars_bterm NVar _ _)  bts
+  | oterm op bts => flat_map (@free_vars_bterm NVar _ Opid )  bts
   end
- with free_vars_bterm {NVar} `{Deq NVar} {gts : GenericTermSig}  (bt : BTerm)
+ with free_vars_bterm {NVar} `{Deq NVar} {Opid:Type}
+    (bt : @BTerm NVar Opid)
   {struct bt} : list NVar :=
   match bt with
-  | bterm  lv nt => remove_nvars lv (free_vars nt)
+  | bterm  lv nt => remove_nvars lv (@free_vars NVar _  Opid nt)
   end.
 
-Fixpoint bound_vars {NVar} `{Deq NVar} {gts : GenericTermSig} (t : NTerm) : list NVar :=
+Fixpoint bound_vars {NVar} `{Deq NVar} {Opid:Type} (t : NTerm) : list NVar :=
   match t with
   | vterm v => []
-  | oterm op bts => flat_map (@bound_vars_bterm NVar _ _)  bts
+  | oterm op bts => flat_map (@bound_vars_bterm NVar _ Opid)  bts
   end
- with bound_vars_bterm {NVar} `{Deq NVar} {gts : GenericTermSig} (bt : BTerm ) 
+ with bound_vars_bterm {NVar} `{Deq NVar} {Opid:Type} (bt : @BTerm NVar Opid) 
   :list NVar :=
   match bt with
   | bterm lv nt => lv ++ bound_vars nt
   end.
 
 Section termsCont.
-Context {NVar VarClass} `{VarType NVar VarClass} {gts : GenericTermSig}.
-Definition all_vars t := free_vars t ++ bound_vars t.
+Context {NVar VarClass} `{VarType NVar VarClass} `{Deq Opid} {gts : GenericTermSig Opid}.
+Definition all_vars (t:@NTerm NVar Opid) : list NVar := free_vars t ++ bound_vars t.
 
 
-Definition closed (t : NTerm) := free_vars t = [].
+Definition closed (t : @NTerm NVar Opid) := free_vars t = [].
 (* Howe's T_0(L) *)
-Definition isprogram (t : NTerm) := closed t # nt_wf t.
+Definition isprogram (t : @NTerm NVar Opid) := closed t # nt_wf t.
 
 End termsCont.
