certicoq/theories/L4_deBruijn/L4_to_L4a.v
@@ -3,6 +3,7 @@ Require Import L4.L4a_to_L5.
 
 Require Import SquiggleEq.export.
 Require Import SquiggleEq.UsefulTypes.
+Require Import SquiggleEq.varImplZ.
 (*
 Require Import SquiggleEq.list.
 Require Import SquiggleEq.LibTactics.
@@ -12,25 +13,99 @@ Require Import SquiggleEq.lmap.
 
 Require Import Coq.Arith.Arith Coq.NArith.BinNat Coq.Strings.String Coq.Lists.List Coq.omega.Omega Coq.Program.Program Coq.micromega.Psatz.
 
-Section VarsOf2Class.
+(*replace in to SquiggleEq and delete here *)
+Fixpoint seq {T:Type} (next: T->T) (start : T) (len : nat) {struct len} : list T :=
+match len with
+| 0 => []
+| S len0 => start :: seq next (next start) len0
+end.
 
-(* see the file SquiggleEq.varImplPeano for an instantiation of NVar *)
-Context {NVar} {deqnvar : Deq NVar} 
-  {vartype: @VarType NVar bool (* 2 species of vars*) _}.
 
+(* make a section so that the notations get cleared *)
+Section Dummy.
+Variable NVar:Type.
+Variable mkVar : N -> NVar.
 
-Notation BTerm := (@BTerm NVar CoqL4GenericTermSig).
-Notation NTerm := (@NTerm NVar CoqL4GenericTermSig).
-Notation oterm := (@oterm NVar CoqL4GenericTermSig).
+Notation BTerm := (@BTerm NVar L4Opid).
+Notation NTerm := (@NTerm NVar L4Opid).
+Notation oterm := (@oterm NVar L4Opid).
 
 Notation push := cons (only parsing).
+
+
+Definition dummyind := Ast.mkInd "" 0%nat.
+
+
+
+(* N.to_nat efficiency? *)
+Fixpoint translate (max : N)(e:exp) : NTerm :=
+match e with
+| Var_e n => vterm (mkVar (max-n-1))
+
+| expression.Lam_e e => 
+    let vn := mkVar max in
+    Lam_e vn (translate (N.succ max) e)
+
+| expression.App_e f a => 
+    App_e (translate max f) (translate max a)
+
+| expression.Let_e e1 e2 => 
+    let vn := mkVar max in
+    Let_e vn (translate max e1) (translate (N.succ max) e2)
+
+| expression.Con_e d el => 
+    Con_e d (translatel max el)
+
+| expression.Fix_e el pn => 
+    let xf := mkVar max in
+    Proj_e (Fix_e xf (translatef (N.succ max) el)) (N.to_nat pn)
+
+| expression.Match_e d _ brl => 
+    Match_e (translate max d) (translateb max brl)
+
+| Ax_e _ => Con_e (dummyind, N.zero) nil (* FIX! *) 
+end
+with translatel (max : N)(e:exps) : list NTerm :=
+match e with
+| enil => []
+| econs h tl => (translate max h)::(translatel max tl)
+end
+with translatef (max:N)(e:efnlst) : list NTerm :=
+match e with
+| eflnil => []
+| eflcons h tl => (translate max h)::(translatef max tl)
+end
+with translateb (max:N)(lb:branches_e) 
+  : list (@branch NVar L4Opid):=
+match lb with
+| brnil_e => []
+| brcons_e d n e tl => 
+    let bvars := map mkVar (seq N.succ max (N.to_nat n)) in 
+    let h := (d, bterm bvars (translate (max+n) e)) in
+    h::(translateb max tl)
+end.
+
+
+End Dummy.
+
+Require Import L6.cps.
+
+(* uservars are supposed to be even, so multiply by 2 x0*)
+Definition L4_to_L4a (e:expression.exp) : (@NTerm cps.var L4Opid) :=
+  translate cps.var (fun n => xO (N.succ_pos n)) (0%N) e.
+
+(*
+(* Delete this module and everything inside it *)
+Module Old.
+Notation NVar := cps.var.
+
+Require Import SquiggleEq.export.
+Require Import L4.expression.
+Require Import L4.L4a_to_L5.
 
 Definition freshVar (lv : list NVar) : NVar :=
 hd nvarx (freshVars 1 (Some true) lv []).
 
-Definition dummyind := Ast.mkInd "" 0%nat.
-
-(* N.to_nat efficiency? *)
 Fixpoint translate (fvars : list NVar)(e:exp) : NTerm :=
 match e with
 | Var_e n => vterm (nth (N.to_nat n) fvars nvarx) (* efficiency? *)
@@ -69,7 +144,7 @@ match e with
 | eflcons h tl => (translate fvars h)::(translatef fvars tl)
 end
 with translateb (fvars : list NVar)(lb:branches_e) 
-  : list (@branch NVar CoqL4GenericTermSig):=
+  : list (@branch NVar L4Opid):=
 match lb with
 | brnil_e => []
 | brcons_e d n e tl => 
@@ -77,24 +152,110 @@ match lb with
     let h := (d, bterm bvars (translate (bvars++fvars) e)) in
     h::(translateb fvars tl)
 end.
+End Old.
+
+Require Import Common.certiClasses.
+Require Export L2.instances.
+Require Export L3.compile.
+Require Export L3.instances.
+Require Import Common.Common.
+Require Import Template.Template.
+
+Quote Recursively Definition p := (3 + 4).
+Quote Recursively Definition id := @id.
+
+Quote Recursively Definition swap := 
+(fun {A B:Type} (p: A  *B) =>
+match p with
+(x,y) => (y,x)
+end).
 
 
-End VarsOf2Class.
 
-Require Import SquiggleEq.varImplZ.
+Section Test.
+Local Instance certiL3_to_L4: 
+  CerticoqTranslation (Program L3.compile.Term) L4.expression.exp  :=
+fun p => Ret (L3_to_L4.translate_program (AstCommon.env p) (main p)).
 
-Require Import L6.cps.
+Require Import Template.Template.
 
-Definition L4_to_L4a (e:expression.exp) : (@NTerm cps.var CoqL4GenericTermSig) :=
-  translate nil e.
 
-(* faster than [L4_to_L4a]. This one exploits the fact that variables are numbers 
-Fixpoint L4_to_L4a_fast (depth : positive (*1 => outside any binder *))
-(e:expression.exp) : NTerm :=
-match e with
-| Var_e n => vterm ((Npos depth) - (n+1))%N
-| _ => vterm xH
-end.
+Open Scope Z_scope.
+Require Import ZArith.
+
+Definition pl4 : L4.expression.exp.
+(let t:= eval compute in (translateTo L4.expression.exp p) in 
+match t with
+|Ret ?xx => exact xx
+end).
+Defined.
+
+Definition id4 : L4.expression.exp.
+(let t:= eval compute in (translateTo L4.expression.exp id) in 
+match t with
+|Ret ?xx => exact xx
+end).
+Defined.
+
+Definition swap4 : L4.expression.exp.
+(let t:= eval compute in (translateTo L4.expression.exp swap) in 
+match t with
+|Ret ?xx => exact xx
+end).
+Defined.
+
+Print swap4.
+Time Eval vm_compute in (L4_to_L4a pl4).
+Time Eval compute in (L4_to_L4a pl4).
+(*0.003 secs*)
+
+Time Eval vm_compute in (Old.translate nil pl4).
+(*0.004 secs*)
+
+Local Opaque Match_e.
+Local Opaque Fix_e.
+Local Opaque Proj_e.
+Local Opaque Con_e.
+Local Opaque Lam_e.
+Local Opaque Let_e.
+Local Opaque App_e.
+
+(*
+Compute runs much slower.
+These Opacity directives cut down the time from 40s to 13.929s
 *)
+Definition pl4a := ltac:(let t:= eval compute in (L4_to_L4a swap4) in exact t).
+Definition pl4aOld := ltac:(let t:= eval compute in (Old.translate nil swap4) in exact t).
 
+Print swap4. (* Why are branches lambdas? *)
+Print pl4a.
+Print pl4aOld.
+
+Local Transparent Match_e.
+Local Transparent Fix_e.
+Local Transparent Proj_e.
+Local Transparent Con_e.
+Local Transparent Lam_e.
+Local Transparent Let_e.
+Local Transparent App_e.
+
+(* fix opacity in squiggleEq *)
+Local Instance deqpos : Deq positive.
+Proof.
+  apply @deqAsSumbool.
+  intros ? ?. unfold DecidableSumbool.
+  decide equality.
+Defined.
+
+Print pl4a.
+Print pl4aOld.
+
+Eval vm_compute in (free_vars pl4aOld).
+Eval vm_compute in (free_vars pl4a).
+
+Print deqpos.
+
+
+End Test.
+*)
 
